mem change

src/computational_monads/simulation_semantics/query_cache/add_fresh_queries.lean
@@ -26,9 +26,9 @@ If the query isn't fresh preserve the value cached in `s'`.
 This behaves like a `⊔` operation if the caches have disjoint `cached_inputs` sets,
 but doesn't in general, so we choose not to implement a `has_sup` typeclass instance. -/
 def add_fresh_queries (cache cache' : query_cache spec) : query_cache spec :=
-{ cache_fn := λ i t, if cache.is_cached i t then cache.lookup i t else cache'.lookup i t,
+{ cache_fn := λ i t, if t ∈ᵢ cache then cache.lookup i t else cache'.lookup i t,
   cached_inputs := cache.cached_inputs ∪ cache'.cached_inputs,
-  mem_cached_inputs := λ x, by split_ifs with hx; simp [hx, mem_cached_inputs_iff_is_cached] }
+  mem_cached_inputs := λ x, by split_ifs with hx; simp [hx, ← mem_iff_mem_cached_inputs'] }
 
 variables (cache cache' : query_cache spec)
 
@@ -36,22 +36,21 @@ variables (cache cache' : query_cache spec)
   cache.cached_inputs ∪ cache'.cached_inputs := rfl
 
 @[simp] lemma lookup_add_fresh_queries (i t) : (cache.add_fresh_queries cache').lookup i t =
-  if cache.is_cached i t then cache.lookup i t else cache'.lookup i t := rfl
+  if t ∈ᵢ cache then cache.lookup i t else cache'.lookup i t := rfl
 
-lemma lookup_add_fresh_queries_of_is_cached {i t} (h : cache.is_cached i t) :
+lemma lookup_add_fresh_queries_of_mem {i t} (h : t ∈ᵢ cache) :
   (cache.add_fresh_queries cache').lookup i t = cache.lookup i t := by simp [h]
 
-@[simp] lemma lookup_add_fresh_queries_of_is_fresh {i t} (h : cache.is_fresh i t) :
-  (cache.add_fresh_queries cache').lookup i t = cache'.lookup i t :=
-by simp [not_is_cached_of_is_fresh _ h]
+lemma lookup_add_fresh_queries_of_not_mem {i t} (h : t ∉ᵢ cache) :
+  (cache.add_fresh_queries cache').lookup i t = cache'.lookup i t := by simp [h]
 
-@[simp] lemma is_fresh_add_fresh_queries_iff (i t) :
-  (cache.add_fresh_queries cache').is_fresh i t ↔ cache.is_fresh i t ∧ cache'.is_fresh i t :=
-by simp [is_fresh_iff_not_mem_cached_inputs, not_or_distrib]
+@[simp] lemma not_mem_add_fresh_queries_iff (i : spec.ι) (t : spec.domain i) :
+  t ∉ᵢ (cache.add_fresh_queries cache') ↔ t ∉ᵢ cache ∧ t ∉ᵢ cache' :=
+by simp [not_mem_iff_not_mem_cached_inputs, not_or_distrib]
 
-@[simp] lemma is_cached_add_fresh_queries_iff (i t) :
-  (cache.add_fresh_queries cache').is_cached i t ↔ cache.is_cached i t ∨ cache'.is_cached i t :=
-by simp [is_cached_iff_mem_cached_inputs]
+@[simp] lemma mem_add_fresh_queries_iff (i : spec.ι) (t : spec.domain i) :
+  t ∈ᵢ (cache.add_fresh_queries cache') ↔ t ∈ᵢ cache ∨ t ∈ᵢ cache' :=
+by simp [mem_iff_mem_cached_inputs]
 
 @[simp] lemma add_fresh_queries_empty (cache : query_cache spec) :
   cache.add_fresh_queries ∅ = cache :=
@@ -68,9 +67,8 @@ begin
   { rw [← h, cached_inputs_add_fresh_queries, finset.mem_union],
     exact or.inr hx },
   { refine query_cache.extₗ (λ i t, ite_eq_left_iff.2 (λ ht, _)),
-    rw [not_is_cached_iff_is_fresh] at ht,
-    exact (lookup_eq_none_of_is_fresh _ (is_fresh_of_cached_inputs_subset_of_is_fresh h ht)).trans
-      (lookup_eq_none_of_is_fresh _ ht).symm }
+    exact (lookup_eq_none_of_not_mem _ (not_mem_of_cached_inputs_subset ht h)).trans
+      (lookup_eq_none_of_not_mem _ ht).symm }
 end
 
 lemma add_fresh_queries_eq_self_of_le {cache cache' : query_cache spec} (h : cache' ≤ cache) :
