src/computational_monads/simulation_semantics/query_cache/basic.lean
@@ -15,10 +15,10 @@ Updates are done using continuation passing with the previous cache.
 
 We also define a number of basic constructors and operations on `query_cache`:
 * `query_cache.lookup` returns the currently cached value.
-* `query_cache.is_fresh` is true iff the given value isn't cached.
-* `query_cache.is_cached` is true iff the given value is cached.
+* `query_cache.mem_inputs` is true iff the given value is cached.
 * `query_cache.cache_query` add a value to the cache.
 * `query_cache.drop_query` removes a value from the cache.
+* `query_cache.empty` has no cached inputs at all.
 -/
 
 /-- Data type representing a cache of oracle queries for a given `oracle_spec`,
@@ -90,6 +90,8 @@ end lookup
 
 section mem
 
+/-- `mem_inputs t cache` means that `t` is in the set of inputs that are cached in `cache`.
+We make the index implicit to enable the use of the notation `t ∈ᵢ cache` and `t ∉ᵢ cache`. -/
 @[derive decidable] def mem_inputs {i : spec.ι} (t : spec.domain i) (cache : query_cache spec) :=
 (sigma.mk i t) ∈ cache.cached_inputs
 
@@ -100,10 +102,17 @@ notation t ` ∉ᵢ `:50 cache:50 := ¬ t ∈ᵢ cache
 lemma mem_iff_mem_cached_inputs (i t) :
   t ∈ᵢ cache ↔ (sigma.mk i t) ∈ cache.cached_inputs := iff.rfl
 
+lemma mem_iff_mem_cached_inputs' (x : Σ i : spec.ι, spec.domain i) :
+  x.2 ∈ᵢ cache ↔ x ∈ cache.cached_inputs := by cases x; refl
+
+/-- An input is cached in `cache` iff `lookup` returns a non-`none` result. -/
 lemma mem_iff_exists_lookup_eq_some (i t) : t ∈ᵢ cache ↔ ∃ u, cache.lookup i t = some u :=
 by rw [mem_iff_mem_cached_inputs, mem_cached_inputs, ← option.is_some_iff_exists, ne.def,
   ← option.is_none_iff_eq_none, ← not_iff_not, option.not_is_some_iff_eq_none,
   option.is_none_iff_eq_none, not_not, apply_eq_lookup]
+
+lemma mem_iff_lookup_ne_none (i t) : t ∈ᵢ cache ↔ cache.lookup i t ≠ none :=
+by simp [option.eq_none_iff_forall_not_mem, mem_iff_exists_lookup_eq_some]
 
 lemma mem_of_lookup_eq_some {i t u} (h : cache.lookup i t = some u) :
   t ∈ᵢ cache := (cache.mem_iff_exists_lookup_eq_some i t).2 ⟨u, h⟩
@@ -167,137 +176,6 @@ end
   some ((cache.lookup i t).get_or_else u) = cache.lookup i t :=
 let ⟨u, hu⟩ := exists_lookup_eq_some_of_mem _ h in by simp [hu]
 
-section is_fresh
-
-/-- `cache.is_fresh i t` means that there isn't any value cached for those inputs. -/
-@[derive decidable]
-def is_fresh (i : spec.ι) (t : spec.domain i) := (cache.lookup i t).is_none = tt
-
-@[simp] lemma lookup_eq_none_iff_is_fresh (i t) : cache.lookup i t = none ↔ cache.is_fresh i t :=
-by simp [is_fresh, option.is_none_iff_eq_none]
-
-@[simp] lemma none_eq_lookup_iff_is_fresh (i t) : none = cache.lookup i t ↔ cache.is_fresh i t :=
-eq_comm.trans (lookup_eq_none_iff_is_fresh cache i t)
-
-lemma is_fresh_of_lookup_eq_none {i t} (h : cache.lookup i t = none) : cache.is_fresh i t :=
-(lookup_eq_none_iff_is_fresh cache i t).1 h
-
-@[simp] lemma lookup_eq_none_of_is_fresh {i t} (h : cache.is_fresh i t) : cache.lookup i t = none :=
-(cache.lookup_eq_none_iff_is_fresh i t).2 h
-
--- TODO: implicitness stuff
-lemma not_is_fresh_of_lookup_eq_some {cache : query_cache spec} {i t u}
-  (h : cache.lookup i t = some u) : ¬ cache.is_fresh i t := by simp [is_fresh, h]
-
-lemma lookup_ne_some_of_is_fresh {i t} (h : cache.is_fresh i t) (u : spec.range i) :
-  cache.lookup i t ≠ some u := by simp [h]
-
-lemma is_fresh_of_is_fresh_of_lookup_eq {i t} (h : cache.is_fresh i t)
-  (h' : cache.lookup i t = cache'.lookup i t) : cache'.is_fresh i t :=
-begin
-  rw [← lookup_eq_none_iff_is_fresh] at ⊢ h,
-  exact h'.symm.trans h
-end
-
-lemma not_mem_cached_inputs_iff_is_fresh (h : Σ i, spec.domain i) :
-  h ∉ cache.cached_inputs ↔ cache.is_fresh h.1 h.2 := by simp [mem_cached_inputs]
-
-lemma is_fresh_iff_not_mem_cached_inputs (i t) :
-  cache.is_fresh i t ↔ (sigma.mk i t) ∉ cache.cached_inputs :=
-by rw [not_mem_cached_inputs_iff_is_fresh]
-
-lemma is_fresh_of_cached_inputs_subset_of_is_fresh {cache cache' : query_cache spec}
-  (h : cache.cached_inputs ⊆ cache'.cached_inputs) {i t}
-  (h' : cache'.is_fresh i t) : cache.is_fresh i t :=
-begin
-  refine by_contra (λ ht, _),
-  rw [is_fresh_iff_not_mem_cached_inputs, not_not] at ht,
-  specialize h ht,
-  rw [is_fresh_iff_not_mem_cached_inputs] at h',
-  exact h' h,
-end
-
-end is_fresh
-
-section is_cached
-
-/-- `cache.is_cached i t` means that there is *some* value cached for the inputs. -/
-@[derive decidable] def is_cached (i : spec.ι) (t : spec.domain i) := ¬ cache.is_fresh i t
-
-@[simp] lemma not_is_cached_iff_is_fresh (i t) : ¬ cache.is_cached i t ↔ cache.is_fresh i t :=
-by rw [is_cached, not_not]
-
-@[simp] lemma not_is_fresh_iff_is_cached (i t) : ¬ cache.is_fresh i t ↔ cache.is_cached i t :=
-by rw [← not_is_cached_iff_is_fresh, not_not]
-
-lemma not_is_cached_of_is_fresh {i t} (h : cache.is_fresh i t) : ¬ cache.is_cached i t :=
-(not_is_cached_iff_is_fresh cache i t).2 h
-
-lemma is_fresh_of_not_is_cached {i t} (h : ¬ cache.is_cached i t) : cache.is_fresh i t :=
-(not_is_cached_iff_is_fresh cache i t).1 h
-
-lemma not_is_fresh_of_is_cached {i t} (h : cache.is_cached i t) : ¬ cache.is_fresh i t :=
-(not_is_fresh_iff_is_cached cache i t).2 h
-
-lemma is_cached_of_not_is_fresh {i t} (h : ¬ cache.is_fresh i t) : cache.is_cached i t :=
-(not_is_fresh_iff_is_cached cache i t).1 h
-
-lemma is_cached_iff_exists_lookup_eq_some (i t) :
-  cache.is_cached i t ↔ ∃ u, cache.lookup i t = some u :=
-by rw [is_cached, is_fresh, option.is_none_iff_eq_none, ← option.not_is_some_iff_eq_none,
-  not_not, option.is_some_iff_exists]
-
-lemma not_is_fresh_iff_exists_lookup_eq_some (i t) :
-  ¬ cache.is_fresh i t ↔ ∃ u, cache.lookup i t = some u :=
-by simp [is_cached_iff_exists_lookup_eq_some]
-
-lemma is_cached_of_lookup_eq_some {i t u} (h : cache.lookup i t = some u) :
-  cache.is_cached i t := (is_cached_iff_exists_lookup_eq_some cache i t).2 ⟨u, h⟩
-
-lemma lookup_eq_some_of_is_cached {i t} (h : cache.is_cached i t) :
-  ∃ u, cache.lookup i t = some u := (cache.is_cached_iff_exists_lookup_eq_some i t).1 h
-
-lemma not_is_cached_of_lookup_eq_none {i t} (h : cache.lookup i t = none) :
-  ¬ cache.is_cached i t := by simp [is_cached_iff_exists_lookup_eq_some, h]
-
-lemma lookup_eq_none_of_not_is_cached {i t} (h : ¬ cache.is_cached i t) :
-  cache.lookup i t = none := lookup_eq_none_of_is_fresh cache (is_fresh_of_not_is_cached _ h)
-
-lemma lookup_ne_none_iff_is_cached (i t) :
-  cache.lookup i t ≠ none ↔ cache.is_cached i t := by simp
-
-lemma lookup_ne_none_iff_exists_lookup_eq_some {i t} :
-  cache.lookup i t ≠ none ↔ ∃ u, cache.lookup i t = some u :=
-by simp [is_cached_iff_exists_lookup_eq_some]
-
-@[simp] lemma some_get_or_else_lookup_of_is_cached {i t u} (h : cache.is_cached i t) :
-  some ((cache.lookup i t).get_or_else u) = cache.lookup i t :=
-let ⟨u, hu⟩ := lookup_eq_some_of_is_cached _ h in by simp [hu]
-
-lemma is_cached_of_is_cached_of_lookup_eq {i t} (h' : cache.is_cached i t)
-  (h : cache.lookup i t = cache'.lookup i t) : cache'.is_cached i t :=
-begin
-  rw [is_cached_iff_exists_lookup_eq_some] at h' ⊢,
-  exact let ⟨u, hu⟩ := h' in ⟨u, h.symm.trans hu⟩
-end
-
-lemma mem_cached_inputs_iff_is_cached (x : Σ i, spec.domain i) :
-  x ∈ cache.cached_inputs ↔ cache.is_cached x.1 x.2 := by simp [mem_cached_inputs]
-
-lemma is_cached_iff_mem_cached_inputs (i t) :
-  cache.is_cached i t ↔ (sigma.mk i t) ∈ cache.cached_inputs :=
-by rw [mem_cached_inputs_iff_is_cached]
-
-lemma is_cached_of_cached_inputs_subset_of_is_cached {cache cache' : query_cache spec}
-  (h : cache.cached_inputs ⊆ cache'.cached_inputs) {i t}
-  (h' : cache.is_cached i t) : cache'.is_cached i t :=
-begin
-  rw [← not_is_fresh_iff_is_cached] at ⊢ h',
-  refine λ ht, h' (is_fresh_of_cached_inputs_subset_of_is_fresh h ht)
-end
-
-end is_cached
-
 end mem
 
 section empty
@@ -320,19 +198,17 @@ instance : inhabited (query_cache spec) := ⟨∅⟩
 
 lemma lookup_empty_ne_some (u : spec.range i) : lookup ∅ i t ≠ some u := by simp
 
-@[simp] lemma is_fresh_empty : is_fresh ∅ i t := by simp [is_fresh]
+@[simp] lemma not_mem_empty : t ∉ᵢ (∅ : query_cache spec) := by simp [mem_iff_mem_cached_inputs]
 
-@[simp] lemma not_is_cached_empty : ¬ is_cached ∅ i t := by simp [is_cached]
-
-@[simp] lemma eq_empty_iff_forall_is_fresh : cache = ∅ ↔ ∀ i t, cache.is_fresh i t :=
+@[simp] lemma eq_empty_iff_forall_not_mem : cache = ∅ ↔ ∀ i (t : spec.domain i), t ∉ᵢ cache :=
 by simp [query_cache.ext_iffₗ]
 
 lemma eq_empty_iff_forall_eq_none : cache = ∅ ↔ ∀ i t, cache.lookup i t = none := by simp
 
-lemma ne_empty_iff_exists_is_cached : cache ≠ ∅ ↔ ∃ i t, cache.is_cached i t := by simp
+lemma ne_empty_iff_exists_mem : cache ≠ ∅ ↔ ∃ i (t : spec.domain i), t ∈ᵢ cache := by simp
 
 lemma ne_empty_iff_exists_eq_some : cache ≠ ∅ ↔ ∃ i t u, cache.lookup i t = some u :=
-by simp [is_cached_iff_exists_lookup_eq_some]
+by simp only [ne_empty_iff_exists_mem, mem_iff_exists_lookup_eq_some]
 
 end empty
 
@@ -350,11 +226,9 @@ def cache_query (i : spec.ι) (t : spec.domain i) (u : spec.range i) (cache : qu
     { induction hi,
       by_cases ht : t = t',
       { simp [ht] },
-      { simp [ht, ne.symm ht, is_cached_iff_mem_cached_inputs] } },
-    { simp [hi, ne.symm hi, is_cached_iff_mem_cached_inputs] }
+      { simp [ht, ne.symm ht, mem_iff_mem_cached_inputs] } },
+    { simp [hi, ne.symm hi, mem_iff_mem_cached_inputs] }
   end }
-
--- variables (i : spec.ι) (t : spec.domain i) (u : spec.range i)
 
 notation `[` i `,` t `↦` u `;` cache `]` := cache_query i t u cache
 
@@ -381,38 +255,30 @@ lemma lookup_cache_query_same_input (i t u) :
 @[simp] lemma cache_query_ne_empty (i t u) : [i, t ↦ u; cache] ≠ ∅ :=
 ne_of_lookup_ne _ _ i t (by simp)
 
-@[simp] lemma is_fresh_cache_query_iff (i t u i' t') :
-  [i, t ↦ u; cache].is_fresh i' t' ↔ cache.is_fresh i' t' ∧
-    (if h : i = i' then h.rec t ≠ t' else true) :=
+@[simp] lemma mem_cache_query_iff (i t u i') (t' : spec.domain i') :
+  t' ∈ᵢ [i, t ↦ u; cache] ↔ t' ∈ᵢ cache ∨ (∃ (h : i = i'), h.rec t = t') :=
 begin
-  simp only [← lookup_eq_none_iff_is_fresh, lookup_cache_query],
-  split_ifs with hi ht,
-  { induction hi, induction ht, simp },
-  { induction hi, simp [ht] },
-  { simp }
+  rw [mem_iff_lookup_ne_none],
+  by_cases hi : i = i',
+  { induction hi,
+    by_cases ht : t = t'; simp [ht] },
+  { simp [hi] }
 end
 
-lemma is_fresh_cache_query_same_index_iff (i t u t') :
-  [i, t ↦ u; cache].is_fresh i t' ↔ cache.is_fresh i t' ∧ t ≠ t' := by simp
+lemma mem_cache_query_same_index_iff (i t u) (t' : spec.domain i) :
+  t' ∈ᵢ [i, t ↦ u; cache] ↔ t' ∈ᵢ cache ∨ t = t' := by simp
 
-lemma not_is_fresh_cache_query_same_input (i t u) : ¬ [i, t ↦ u; cache].is_fresh i t := by simp
+lemma mem_cache_query_diff_index_iff {i i'} (hi : i ≠ i') (t u) (t' : spec.domain i') :
+  t' ∈ᵢ [i, t ↦ u; cache] ↔ t' ∈ᵢ cache := by simp [hi]
 
-@[simp] lemma is_cached_cache_query_iff (i t u i' t') :
-  [i, t ↦ u; cache].is_cached i' t' ↔ cache.is_cached i' t' ∨
-    (if h : i = i' then h.rec t = t' else false) :=
-begin
-  rw [← not_is_fresh_iff_is_cached, is_fresh_cache_query_iff,
-    not_and_distrib, not_is_fresh_iff_is_cached],
-  split_ifs; simp
-end
+lemma mem_cache_query_same_input (i t u) :
+  t ∈ᵢ [i, t ↦ u; cache] := by simp
 
-lemma is_cached_cache_query_same_index_iff (i t u t') :
-  [i, t ↦ u; cache].is_cached i t' ↔ cache.is_cached i t' ∨ t = t' := by simp
+lemma mem_cache_query_diff_input_iff (i) {t t'} (ht : t ≠ t') (u) :
+  t' ∈ᵢ [i, t ↦ u; cache] ↔ t' ∈ᵢ cache := by simp [ht]
 
-lemma is_cached_cache_query_same_input (i t u) : [i, t ↦ u; cache].is_cached i t := by simp
-
-lemma cache_query_inj_of_is_fresh {cache cache' : query_cache spec} {i t}
-  (h : cache.is_fresh i t) (h' : cache'.is_fresh i t) (u) :
+lemma cache_query_inj_of_not_mem {cache cache' : query_cache spec}
+  {i t} (h : t ∉ᵢ cache) (h' : t ∉ᵢ cache') (u) :
   [i, t ↦ u; cache] = [i, t ↦ u; cache'] ↔ cache = cache' :=
 begin
   simp only [query_cache.ext_iffₗ],
@@ -478,44 +344,30 @@ lemma lookup_drop_query_same_input (i t) : (cache.drop_query i t).lookup i t = n
 lemma lookup_drop_query_diff_input (i) {t t'} (ht : t ≠ t'):
   (cache.drop_query i t).lookup i t' = cache.lookup i t' := by simp [ht]
 
-@[simp] lemma drop_query_of_is_fresh {i t} (h : cache.is_fresh i t) :
-  cache.drop_query i t = cache :=
+@[simp] lemma drop_query_of_not_mem {i t} (h : t ∉ᵢ cache) : cache.drop_query i t = cache :=
 query_cache.extₗ_induction (λ i t u, cache.drop_query i t)
   cache i t default (by simp [h]) (λ t ht, by simp [ht]) (λ i t hi, by simp [hi])
 
-@[simp] lemma is_fresh_drop_query_iff (i t i' t') :
-  (cache.drop_query i t).is_fresh i' t' ↔ cache.is_fresh i' t' ∨ ∃ (h : i = i'), h.rec t = t' :=
+@[simp] lemma mem_drop_query_iff (i t i') (t' : spec.domain i') :
+  t' ∈ᵢ (cache.drop_query i t) ↔ t' ∈ᵢ cache ∧ (if h : i = i' then h.rec t ≠ t' else true) :=
 begin
-  refine ⟨λ h, _, λ h, (lookup_eq_none_iff_is_fresh _ _ _).1 (h.rec_on (λ h', _) _)⟩,
-  { by_cases hi : i = i',
-    { induction hi,
-      by_cases ht : t = t',
-      { exact or.inr ⟨rfl, ht⟩ },
-      { simp_rw [← lookup_eq_none_iff_is_fresh, lookup_drop_query_same_index, ht,
-          if_false, lookup_eq_none_iff_is_fresh] at h,
-        exact or.inl h } },
-    { refine or.inl _,
-      simpa [lookup_drop_query, hi, if_false] using ((lookup_eq_none_iff_is_fresh _ _ _).2 h) } },
-  { { by_cases hi : i = i',
-      { induction hi,
-        by_cases ht : t = t',
-        { simp [ht, lookup_drop_query_same_input _ _ _] },
-        { simpa [lookup_drop_query_diff_input _ _ ht] } },
-      { simpa [lookup_drop_query_diff_index _ hi] } } },
-  { rintro ⟨rfl, rfl⟩,
-    simp }
+  rw [mem_iff_lookup_ne_none],
+  by_cases hi : i = i',
+  { induction hi,
+    by_cases ht : t = t'; simp [ht] },
+  { simp [hi] }
 end
 
-lemma is_fresh_drop_query_iff_same_index (i t t') :
-  (cache.drop_query i t).is_fresh i t' ↔ cache.is_fresh i t' ∨ t = t' := by simp
+lemma mem_drop_query_same_index_iff (i t) (t' : spec.domain i) :
+  t' ∈ᵢ (cache.drop_query i t) ↔ t' ∈ᵢ cache ∧ t ≠ t' := by simp
 
-lemma is_fresh_drop_query_iff_diff_index {i i'} (h : i ≠ i') (t t') :
-  (cache.drop_query i t).is_fresh i' t' ↔ cache.is_fresh i' t' := by simp [h]
+lemma mem_drop_query_diff_index_iff {i i'} (hi : i ≠ i') (t) (t' : spec.domain i') :
+  t' ∈ᵢ (cache.drop_query i t) ↔ t' ∈ᵢ cache := by simp [hi]
 
-lemma is_fresh_drop_query_same_input (i t) : (cache.drop_query i t).is_fresh i t := by simp
+lemma not_mem_drop_query_same_input (i t) : t ∉ᵢ (cache.drop_query i t) := by simp
 
-lemma is_fresh_drop_query_iff_diff_input (i) {t t'} (h : t ≠ t') :
-  (cache.drop_query i t).is_fresh i t' ↔ cache.is_fresh i t' := by simp [h]
+lemma mem_drop_query_diff_input_iff (i) {t t'} (ht : t ≠ t') :
+  t' ∈ᵢ (cache.drop_query i t) ↔ t' ∈ᵢ cache := by simp [ht]
 
 @[simp] lemma drop_query_empty (i : spec.ι) (t) : drop_query i t ∅ = ∅ := by simp
 
@@ -526,8 +378,8 @@ section drop_query_cache_query
 /-- Adding a query to the cache and then dropping a query commutes to dropping and then adding,
 unless the inputs being cached are the same as the one being dropped. -/
 @[simp] lemma drop_query_cache_query (i t u i' t') :
-  [i, t ↦ u; cache].drop_query i' t' = if h : i = i' then (if h.rec t = t' then cache.drop_query i' t'
-    else [i, t ↦ u; cache.drop_query i' t']) else [i, t ↦ u; cache.drop_query i' t'] :=
+  [i, t ↦ u; cache].drop_query i' t' = if ∃ (h : i = i'), h.rec t = t'
+    then cache.drop_query i' t' else [i, t ↦ u; cache.drop_query i' t'] :=
 begin
   refine query_cache.extₗ (λ i'' t'', _),
   by_cases hi : i = i',
@@ -570,8 +422,8 @@ end drop_query_cache_query
 section cache_query_drop_query
 
 lemma cache_query_drop_query (i t u i' t') :
-  [i, t ↦ u; cache.drop_query i' t'] = if h : i = i' then (if h.rec t = t' then [i, t ↦ u; cache]
-    else [i, t ↦ u; cache].drop_query i' t') else [i, t ↦ u; cache].drop_query i' t' :=
+  [i, t ↦ u; cache.drop_query i' t'] = if ∃ (h : i = i'), h.rec t = t'
+    then [i, t ↦ u; cache] else [i, t ↦ u; cache].drop_query i' t' :=
 begin
   refine query_cache.extₗ (λ i'' t'', _),
   by_cases hi : i = i',
@@ -597,16 +449,16 @@ begin
       { simp [hi, hi', hi''] } } }
 end
 
-@[simp] lemma cache_query_drop_query_same_index (i t u t') :
+lemma cache_query_drop_query_same_index (i t u t') :
   [i, t ↦ u; cache.drop_query i t'] = if t = t' then [i, t ↦ u; cache]
     else [i, t ↦ u; cache].drop_query i t' :=
-by simp only [cache_query_drop_query, dif_pos]
+by simp only [cache_query_drop_query, eq_self_iff_true, exists_true_left]
 
 /-- Adding a value to a cache after removing a value for the same inputs is the same as just
 caching it into the original cache, since adding new values replaces old ones. -/
 @[simp] lemma cache_query_drop_query_same_input (i t u) :
   [i, t ↦ u; cache.drop_query i t] = [i, t ↦ u; cache] :=
-by simp only [cache_query_drop_query, eq_self_iff_true, if_true, dite_eq_ite]
+by simp only [cache_query_drop_query, eq_self_iff_true, exists_true_left, if_true]
 
 end cache_query_drop_query
 
@@ -623,74 +475,75 @@ def singleton (i : spec.ι) (t : spec.domain i) (u : spec.range i) := [i, t ↦ 
 
 notation `[` i `,` t `↦` u `]` := singleton i t u
 
-variables (i : spec.ι) (t : spec.domain i) (u : spec.range i)
+-- variables (i : spec.ι) (t : spec.domain i) (u : spec.range i)
 
-lemma singleton.def : [i, t ↦ u] = [i, t ↦ u; ∅] := rfl
+lemma singleton.def (i t) (u : spec.range i) : [i, t ↦ u] = [i, t ↦ u; ∅] := rfl
 
-lemma lookup_singleton (i' : spec.ι) (t' : spec.domain i') :
+lemma lookup_singleton (i : spec.ι) (t u i' t') :
   [i, t ↦ u].lookup i' t' = if h : i = i' then
     (if h.rec t = t' then some (h.rec u) else none) else none := rfl
 
-@[simp] lemma lookup_singleton_same_index (t' : spec.domain i) :
+@[simp] lemma lookup_singleton_same_index (i : spec.ι) (t u t') :
   [i, t ↦ u].lookup i t' = if t = t' then some u else none := by simp [lookup_singleton]
 
-@[simp] lemma lookup_singleton_diff_index (i' : spec.ι) (t' : spec.domain i') (h : i ≠ i') :
-  [i, t ↦ u].lookup i' t' = none := by simp [lookup_singleton, h]
+@[simp] lemma lookup_singleton_diff_index {i i' : spec.ι} (hi : i ≠ i') (t u t') :
+  [i, t ↦ u].lookup i' t' = none := by simp [lookup_singleton, hi]
 
-lemma lookup_singleton_same_input :
+lemma lookup_singleton_same_input (i : spec.ι) (t u) :
   [i, t ↦ u].lookup i t = some u := by simp
 
-@[simp] lemma lookup_singleton_diff_input (t' : spec.domain i) (h : t ≠ t') :
-  [i, t ↦ u].lookup i t' = none := by simp [h]
+@[simp] lemma lookup_singleton_diff_input (i : spec.ι) {t t'} (ht : t ≠ t') (u) :
+  [i, t ↦ u].lookup i t' = none := by simp [ht]
 
-@[simp] lemma cached_inputs_singleton : [i, t ↦ u].cached_inputs = {⟨i, t⟩} := rfl
+@[simp] lemma cached_inputs_singleton (i : spec.ι) (t u) :
+  [i, t ↦ u].cached_inputs = {⟨i, t⟩} := rfl
 
-lemma lookup_singleton_eq_some_iff (i' : spec.ι) (t' : spec.domain i')
-  (u' : spec.range i') : [i, t ↦ u].lookup i' t' = some u' ↔
+lemma lookup_singleton_eq_some_iff (i : spec.ι) (t u i' t' u') :
+  [i, t ↦ u].lookup i' t' = some u' ↔
     ∃ (h : i = i'), h.rec t = t' ∧ h.rec u = u' :=
 by simp [lookup_singleton, dite_eq_iff, ite_eq_iff]
 
-lemma lookup_singleton_eq_some_iff_same_index (t' : spec.domain i) (u' : spec.range i) :
+lemma lookup_singleton_eq_some_iff_same_index (i : spec.ι) (t u t' u') :
   [i, t ↦ u].lookup i t' = some u' ↔ t = t' ∧ u = u' :=
 by simp [lookup_singleton_eq_some_iff, ite_eq_iff]
 
-lemma lookup_singleton_eq_some_iff_same_input (u' : spec.range i) :
+lemma lookup_singleton_eq_some_iff_same_input (i : spec.ι) (t u u') :
   [i, t ↦ u].lookup i t = some u' ↔ u = u' := by simp
 
-lemma singleton_ne_empty : [i, t ↦ u] ≠ ∅ := cache_query_ne_empty ∅ i t u
+lemma singleton_ne_empty (i : spec.ι) (t u) : [i, t ↦ u] ≠ ∅ := cache_query_ne_empty ∅ i t u
 
-@[simp] lemma is_fresh_singleton_iff (i' : spec.ι) (t' : spec.domain i') :
-  [i, t ↦ u].is_fresh i' t' ↔ if h : i = i' then h.rec t ≠ t' else true := by simp [singleton.def]
+@[simp] lemma mem_singleton_iff (i : spec.ι) (t u i' t') :
+  t' ∈ᵢ [i, t ↦ u] ↔ ∃ (h : i = i'), h.rec t = t' := by simp [singleton.def]
 
-lemma is_fresh_singleton_iff_same_index (t' : spec.domain i) :
-  [i, t ↦ u].is_fresh i t' ↔ t ≠ t' := by simp
+lemma mem_singleton_iff_same_index (i : spec.ι) (t u t') :
+  t' ∈ᵢ [i, t ↦ u] ↔ t = t' := by simp
 
-lemma is_fresh_singleton_diff_index (i' : spec.ι) (t' : spec.domain i') (h : i ≠ i') :
-  [i, t ↦ u].is_fresh i' t' := by simp [h]
+lemma not_mem_singleton_diff_index {i i' : spec.ι} (hi : i ≠ i') (t u) (t' : spec.domain i') :
+  t' ∉ᵢ [i, t ↦ u] := by simp [hi]
 
-lemma not_is_fresh_singleton_same_input : ¬ [i, t ↦ u].is_fresh i t := by simp
+lemma mem_singleton_same_input (i : spec.ι) (t u) : t ∈ᵢ [i, t ↦ u] := by simp
 
-lemma is_fresh_singleton_diff_input (t' : spec.domain i) (h : t ≠ t') :
-  [i, t ↦ u].is_fresh i t' := by simp [h]
+lemma not_mem_singleton_diff_input (i : spec.ι) {t t'} (ht : t ≠ t') (u) :
+  t' ∉ᵢ [i, t ↦ u] := by simp [ht]
 
-@[simp] lemma drop_query_singleton (i' : spec.ι) (t' : spec.domain i') :
-  [i, t ↦ u].drop_query i' t' = if h : i = i' then (if h.rec t = t' then ∅
-    else [i, t ↦ u]) else [i, t ↦ u] :=
+@[simp] lemma drop_query_singleton (i : spec.ι) (t u i' t') :
+  [i, t ↦ u].drop_query i' t' = if ∃ (h : i = i'), h.rec t = t' then ∅ else [i, t ↦ u] :=
 by simp [singleton.def]
 
-lemma drop_query_singleton_same_index (t' : spec.domain i) :
+lemma drop_query_singleton_same_index (i : spec.ι) (t u t') :
   [i, t ↦ u].drop_query i t' = if t = t' then ∅ else [i, t ↦ u] := by simp
 
-lemma drop_query_singleton_diff_index (i' : spec.ι) (t' : spec.domain i') (h : i ≠ i') :
-  [i, t ↦ u].drop_query i' t' = [i, t ↦ u] := by simp [h]
+lemma drop_query_singleton_diff_index {i i' : spec.ι} (hi : i ≠ i') (t u t') :
+  [i, t ↦ u].drop_query i' t' = [i, t ↦ u] := by simp [hi]
 
-lemma drop_query_singleton_same_input : [i, t ↦ u].drop_query i t = ∅ := by simp
+lemma drop_query_singleton_same_input (i : spec.ι) (t u) :
+  [i, t ↦ u].drop_query i t = ∅ := by simp
 
-lemma drop_query_singleton_diff_input (t' : spec.domain i) (h : t ≠ t') :
-  [i, t ↦ u].drop_query i t' = [i, t ↦ u] := by simp [h]
+lemma drop_query_singleton_diff_input (i : spec.ι) {t t'} (ht : t ≠ t') (u) :
+  [i, t ↦ u].drop_query i t' = [i, t ↦ u] := by simp [ht]
 
-lemma lookup_cache_query_eq_lookup_singleton (i' : spec.ι) (t' : spec.domain i')
-  (h : cache.is_fresh i' t') : [i, t ↦ u; cache].lookup i' t' = [i, t ↦ u].lookup i' t' :=
+lemma lookup_cache_query_eq_lookup_singleton (i : spec.ι) (t u) {i' t'} (h : t' ∉ᵢ cache) :
+  [i, t ↦ u; cache].lookup i' t' = [i, t ↦ u].lookup i' t' :=
 begin
   by_cases hi : i = i',
   { induction hi,
