src/computational_monads/simulation_semantics/query_cache/get_or_else.lean
@@ -36,132 +36,130 @@ section ite
 variables (i : spec.ι) (t : spec.domain i) (ou : oracle_comp spec' (spec.range i))
 
 lemma get_or_else_eq_ite : cache.get_or_else i t ou =
-  if cache.is_fresh i t then ou >>= λ u, return (u, [i, t ↦ u; cache])
-    else return ((cache.lookup i t).get_or_else default, cache) :=
+  if t ∈ᵢ cache then return ((cache.lookup i t).get_or_else default, cache)
+    else ou >>= λ u, return (u, [i, t ↦ u; cache]) :=
 begin
   split_ifs with h,
-  { simp [get_or_else, lookup_eq_none_of_is_fresh _ h] },
-  { rw [not_is_fresh_iff_exists_lookup_eq_some] at h,
+  { rw [mem_iff_exists_lookup_eq_some] at h,
     obtain ⟨u, hu⟩ := h,
-    simp [get_or_else, hu] }
+    simp [get_or_else, hu] },
+  { simp [get_or_else, lookup_eq_none_of_not_mem _ h] }
 end
 
 lemma support_get_or_else : (cache.get_or_else i t ou).support =
-  if cache.is_fresh i t then (λ u, (u, [i, t ↦ u; cache])) '' ou.support else
-    {((cache.lookup i t).get_or_else default, cache)} :=
+  if t ∈ᵢ cache then {((cache.lookup i t).get_or_else default, cache)}
+    else (λ u, (u, [i, t ↦ u; cache])) '' ou.support :=
 by simp [get_or_else_eq_ite]
 
 lemma mem_support_get_or_else_iff (x : spec.range i × query_cache spec) :
   x ∈ (cache.get_or_else i t ou).support ↔
-    if cache.is_fresh i t then x.1 ∈ ou.support ∧ [i, t ↦ x.1; cache] = x.2 else
-      cache.lookup i t = some x.1 ∧ x.2 = cache :=
+    if t ∈ᵢ cache then cache.lookup i t = some x.1 ∧ x.2 = cache
+      else x.1 ∈ ou.support ∧ [i, t ↦ x.1; cache] = x.2 :=
 begin
   split_ifs with h,
+  { obtain ⟨u, hu⟩ := exists_lookup_eq_some_of_mem _ h,
+    simp [get_or_else_eq_ite, h, prod.eq_iff_fst_eq_snd_eq, hu, eq_comm] },
   { simp [get_or_else_eq_ite, h],
     refine ⟨λ h', _, λ h', _⟩,
     { obtain ⟨u, hu⟩ := h',
       rw [prod.eq_iff_fst_eq_snd_eq] at hu,
       exact ⟨hu.2.1 ▸ hu.1, hu.2.1 ▸ hu.2.2⟩ },
     { exact ⟨x.1, h'.1, prod.eq_iff_fst_eq_snd_eq.2 ⟨rfl, h'.2⟩⟩ } },
-  { obtain ⟨u, hu⟩ := lookup_eq_some_of_is_cached _ (is_cached_of_not_is_fresh _ h),
-    simp [get_or_else_eq_ite, h, prod.eq_iff_fst_eq_snd_eq, hu, eq_comm] }
 end
 
 lemma eval_dist_get_or_else : ⁅cache.get_or_else i t ou⁆ =
-  if cache.is_fresh i t then ⁅ou⁆.map (λ u, (u, [i, t ↦ u; cache]))
-    else pmf.pure ((cache.lookup i t).get_or_else default, cache) :=
+  if t ∈ᵢ cache then pmf.pure ((cache.lookup i t).get_or_else default, cache)
+    else ⁅ou⁆.map (λ u, (u, [i, t ↦ u; cache])) :=
 by simp [get_or_else_eq_ite]
 
 lemma prob_output_get_or_else (x) : ⁅= x | cache.get_or_else i t ou⁆ =
-  if cache.is_fresh i t then ⁅= x | ou >>= λ u, return (u, [i, t ↦ u; cache])⁆
-    else ⁅= x | return' !spec'! ((cache.lookup i t).get_or_else default, cache)⁆ :=
+  if t ∈ᵢ cache then ⁅= x | return' !spec'! ((cache.lookup i t).get_or_else default, cache)⁆
+    else ⁅= x | ou >>= λ u, return (u, [i, t ↦ u; cache])⁆ :=
 by simp [get_or_else_eq_ite]
 
 lemma prob_event_get_or_else (e) : ⁅e | cache.get_or_else i t ou⁆ =
-  if cache.is_fresh i t then ⁅e | ou >>= λ u, return (u, [i, t ↦ u; cache])⁆
-    else ⁅e | return' !spec! ((cache.lookup i t).get_or_else default, cache)⁆ :=
+  if t ∈ᵢ cache then ⁅e | return' !spec! ((cache.lookup i t).get_or_else default, cache)⁆
+    else ⁅e | ou >>= λ u, return (u, [i, t ↦ u; cache])⁆ :=
 by simp [get_or_else_eq_ite]
 
-lemma get_or_else_dist_equiv : cache.get_or_else i t ou ≃ₚ
-  if cache.is_fresh i t then ou >>= λ u, return (u, [i, t ↦ u; cache]) else
-    return ((cache.lookup i t).get_or_else default, cache) :=
+@[simp_dist_equiv] lemma get_or_else_dist_equiv : cache.get_or_else i t ou ≃ₚ
+  if t ∈ᵢ cache then return ((cache.lookup i t).get_or_else default, cache)
+    else ou >>= λ u, return (u, [i, t ↦ u; cache]) :=
 by rw [get_or_else_eq_ite]
-
--- lemma get_or_else_dist_equiv_get_or_else
 
 end ite
 
-section is_fresh
+section mem
 
 variables {i : spec.ι} {t : spec.domain i} (ou : oracle_comp spec' (spec.range i))
 
-@[simp] lemma get_or_else_of_is_fresh (h : cache.is_fresh i t) :
-  cache.get_or_else i t ou = ou >>= λ u, return (u, [i, t ↦ u; cache]) :=
-by simp [get_or_else, h]
-
-lemma support_get_or_else_of_is_fresh (h : cache.is_fresh i t) :
-  (cache.get_or_else i t ou).support = (λ u, (u, [i, t ↦ u; cache])) '' ou.support :=
-by simp [h]
-
-lemma mem_support_get_or_else_iff_of_is_fresh (h : cache.is_fresh i t)
-  (x : spec.range i × query_cache spec) : x ∈ (cache.get_or_else i t ou).support ↔
-    x.1 ∈ ou.support ∧ [i, t ↦ x.1; cache] = x.2 :=
-by simp only [mem_support_get_or_else_iff, h, if_true]
-
-lemma eval_dist_get_or_else_of_is_fresh (h : cache.is_fresh i t) :
-  ⁅cache.get_or_else i t ou⁆ = ⁅ou⁆.map (λ u, (u, [i, t ↦ u; cache])) :=
-by simp [h]
-
-lemma prob_output_get_or_else_of_is_fresh (h : cache.is_fresh i t) (x) :
-  ⁅= x | cache.get_or_else i t ou⁆ = ⁅= x | ou >>= λ u, return (u, [i, t ↦ u; cache])⁆ :=
-by simp [h]
-
-lemma prob_event_get_or_else_of_is_fresh (h : cache.is_fresh i t) (e) :
-  ⁅e | cache.get_or_else i t ou⁆ = ⁅e | ou >>= λ u, return (u, [i, t ↦ u; cache])⁆ :=
-by simp [h]
-
-lemma get_or_else_dist_equiv_of_is_fresh (h : cache.is_fresh i t) :
-  cache.get_or_else i t ou ≃ₚ ou >>= λ u, return (u, [i, t ↦ u; cache]) :=
-by rw [get_or_else_of_is_fresh _ _ h]
-
-end is_fresh
-
-section is_cached
-
-variables {i : spec.ι} {t : spec.domain i} (ou : oracle_comp spec' (spec.range i))
-
-@[simp] lemma get_or_else_of_is_cached (h : cache.is_cached i t) :
+@[simp] lemma get_or_else_of_mem (h : t ∈ᵢ cache) :
   cache.get_or_else i t ou = return ((cache.lookup i t).get_or_else default, cache) :=
-by simp only [get_or_else_eq_ite, ← not_is_cached_iff_is_fresh, h, not_true, if_false]
+by simp only [get_or_else_eq_ite, h, if_true]
 
-lemma support_get_or_else_of_is_cached (h : cache.is_cached i t) :
+lemma support_get_or_else_of_mem (h : t ∈ᵢ cache) :
   (cache.get_or_else i t ou).support = {((cache.lookup i t).get_or_else default, cache)} :=
 by simp [h]
 
-lemma mem_support_get_or_else_iff_of_is_cached (h : cache.is_cached i t)
+lemma mem_support_get_or_else_iff_of_mem (h : t ∈ᵢ cache)
   (x : spec.range i × query_cache spec) : x ∈ (cache.get_or_else i t ou).support ↔
     cache.lookup i t = some x.1 ∧ x.2 = cache :=
-by simp only [(not_is_fresh_of_is_cached _ h), mem_support_get_or_else_iff, if_false]
+by simp only [h, mem_support_get_or_else_iff, if_true]
 
-lemma eval_dist_get_or_else_of_is_cached (h : cache.is_cached i t) :
+lemma eval_dist_get_or_else_of_mem (h : t ∈ᵢ cache) :
   ⁅cache.get_or_else i t ou⁆ = pmf.pure ((cache.lookup i t).get_or_else default, cache) :=
 by simp [h]
 
-lemma prob_output_get_or_else_of_is_cached (h : cache.is_cached i t) (x) :
+lemma prob_output_get_or_else_of_mem (h : t ∈ᵢ cache) (x) :
   ⁅= x | cache.get_or_else i t ou⁆ =
     ⁅= x | return' !spec'! ((cache.lookup i t).get_or_else default, cache)⁆ :=
 by simp [h]
 
-lemma prob_event_get_or_else_of_is_cached (h : cache.is_cached i t) (e) :
+lemma prob_event_get_or_else_of_mem (h : t ∈ᵢ cache) (e) :
   ⁅e | cache.get_or_else i t ou⁆ =
     ⁅e | return' !spec! ((cache.lookup i t).get_or_else default, cache)⁆ :=
 by simp [h]
 
-lemma get_or_else_dist_equiv_of_is_cached (h : cache.is_cached i t) :
+lemma get_or_else_dist_equiv_of_mem (h : t ∈ᵢ cache) :
   cache.get_or_else i t ou ≃ₚ return' !spec! ((cache.lookup i t).get_or_else default, cache) :=
 by simp [h]
 
-end is_cached
+end mem
+
+section not_mem
+
+variables {i : spec.ι} {t : spec.domain i} (ou : oracle_comp spec' (spec.range i))
+
+@[simp] lemma get_or_else_of_not_mem (h : t ∉ᵢ cache) :
+  cache.get_or_else i t ou = ou >>= λ u, return (u, [i, t ↦ u; cache]) :=
+by simp [get_or_else, h]
+
+lemma support_get_or_else_of_not_mem (h : t ∉ᵢ cache) :
+  (cache.get_or_else i t ou).support = (λ u, (u, [i, t ↦ u; cache])) '' ou.support :=
+by simp [h]
+
+lemma mem_support_get_or_else_iff_of_not_mem (h : t ∉ᵢ cache)
+  (x : spec.range i × query_cache spec) : x ∈ (cache.get_or_else i t ou).support ↔
+    x.1 ∈ ou.support ∧ [i, t ↦ x.1; cache] = x.2 :=
+by simp only [mem_support_get_or_else_iff, h, if_false]
+
+lemma eval_dist_get_or_else_of_not_mem (h : t ∉ᵢ cache) :
+  ⁅cache.get_or_else i t ou⁆ = ⁅ou⁆.map (λ u, (u, [i, t ↦ u; cache])) :=
+by simp [h]
+
+lemma prob_output_get_or_else_of_not_mem (h : t ∉ᵢ cache) (x) :
+  ⁅= x | cache.get_or_else i t ou⁆ = ⁅= x | ou >>= λ u, return (u, [i, t ↦ u; cache])⁆ :=
+by simp [h]
+
+lemma prob_event_get_or_else_of_not_mem (h : t ∉ᵢ cache) (e) :
+  ⁅e | cache.get_or_else i t ou⁆ = ⁅e | ou >>= λ u, return (u, [i, t ↦ u; cache])⁆ :=
+by simp [h]
+
+lemma get_or_else_dist_equiv_of_not_mem (h : t ∉ᵢ cache) :
+  cache.get_or_else i t ou ≃ₚ ou >>= λ u, return (u, [i, t ↦ u; cache]) :=
+by rw [get_or_else_of_not_mem _ _ h]
+
+end not_mem
 
 section lookup_eq_some
 
@@ -199,7 +197,7 @@ section empty
 variables (i : spec.ι) (t : spec.domain i) (ou : oracle_comp spec' (spec.range i))
 
 @[simp] lemma get_or_else_empty : get_or_else ∅ i t ou = do {u ← ou, return (u, [i, t ↦ u])} :=
-by simp [is_fresh_empty i t, singleton.def]
+by simp [not_mem_empty i t, singleton.def]
 
 end empty
 
@@ -215,17 +213,17 @@ lemma lookup_snd_eq_of_mem_support_get_or_else (i' : spec.ι) (t' : spec.domain 
 begin
   by_cases hi : i = i',
   { induction hi,
-    by_cases ht : cache.is_fresh i t,
-    { rw [mem_support_get_or_else_iff_of_is_fresh _ _ ht] at h,
-      simp [← h.2] },
-    { simp [is_cached_of_not_is_fresh _ ht] at h,
-      simp [h, is_cached_of_not_is_fresh _ ht],
-      split_ifs with htt; simp [htt] } },
-  { by_cases ht : cache.is_fresh i t,
-    { rw [mem_support_get_or_else_iff_of_is_fresh _ _ ht] at h,
-      simp [← h.2, hi] },
-    { simp [is_cached_of_not_is_fresh _ ht] at h,
-      simp [h, is_cached_of_not_is_fresh _ ht, hi] } }
+    by_cases ht : t ∈ᵢ cache,
+    { simp [ht] at h,
+      simp [h, ht],
+      split_ifs with htt; simp [htt] },
+    { rw [mem_support_get_or_else_iff_of_not_mem _ _ ht] at h,
+      simp [← h.2] } },
+  { by_cases ht : t ∈ᵢ cache,
+    { simp [ht] at h,
+      simp [h, ht, hi] },
+    { rw [mem_support_get_or_else_iff_of_not_mem _ _ ht] at h,
+      simp [← h.2, hi] } }
 end
 
 lemma lookup_snd_eq_of_mem_support_get_or_else_same_index (t' : spec.domain i)
@@ -246,9 +244,9 @@ lemma lookup_snd_eq_of_mem_support_get_or_else_diff_input (t' : spec.domain i) (
   (h : x ∈ (cache.get_or_else i t ou).support) : x.2.lookup i t' = cache.lookup i t' :=
 by simp [lookup_snd_eq_of_mem_support_get_or_else _ _ _ _ h, ht]
 
-lemma is_cached_of_mem_support_get_or_else
-  (h : x ∈ (cache.get_or_else i t ou).support) : x.2.is_cached i t :=
-is_cached_of_lookup_eq_some _ (lookup_snd_eq_of_mem_support_get_or_else_same_input _ _ h)
+lemma mem_of_mem_support_get_or_else
+  (h : x ∈ (cache.get_or_else i t ou).support) : t ∈ᵢ x.2 :=
+mem_of_lookup_eq_some _ (lookup_snd_eq_of_mem_support_get_or_else_same_input _ _ h)
 
 end lookup
 
@@ -259,11 +257,11 @@ variables {i : spec.ι} {t : spec.domain i} {ou : oracle_comp spec' (spec.range 
 
 lemma le_of_mem_support_get_or_else (h : x ∈ (cache.get_or_else i t ou).support) : cache ≤ x.2 :=
 begin
-  by_cases ht : cache.is_fresh i t,
-  { rw [mem_support_get_or_else_iff_of_is_fresh _ _ ht] at h,
+  by_cases ht : t ∈ᵢ cache,
+  { rw [mem_support_get_or_else_iff_of_mem _ _ ht] at h,
+    refine h.2 ▸ le_rfl },
+  { rw [mem_support_get_or_else_iff_of_not_mem _ _ ht] at h,
     refine h.2 ▸ le_cache_query_self _ _ _ _ },
-  { rw [mem_support_get_or_else_iff_of_is_cached _ _ (is_cached_of_not_is_fresh _ ht)] at h,
-    refine h.2 ▸ le_rfl }
 end
 
 lemma le_of_mem_support_snd_map_get_or_else (cache' : query_cache spec)
@@ -280,17 +278,16 @@ lemma fst_map_get_or_else_dist_equiv_fst_map_get_or_else
   (h : cache.lookup i t = cache'.lookup i t) :
   prod.fst <$> cache.get_or_else i t ou ≃ₚ prod.fst <$> cache'.get_or_else i t ou :=
 begin
-  by_cases h' : cache.is_cached i t,
+  by_cases h' : t ∈ᵢ cache,
   {
 
-    have : cache'.is_cached i t := _,
+    have : t ∈ᵢ cache := sorry,
     simp [h', this, h],
     sorry,
   },
   {
-    have h1 : cache.is_fresh i t := sorry,
-    have : cache'.is_fresh i t := sorry,
-    simp [h, h1, this],
+    have : t ∉ᵢ cache' := sorry,
+    simp [h, h', this],
   }
 end
 
@@ -364,9 +361,6 @@ lemma get_or_else_bind_get_or_else_dist_equiv_same_input (t' : spec.domain i) :
     cache.get_or_else i t' ou :=
 begin
   sorry
-  -- refine bind_dist_equiv_left _ _ (λ x hx, _),
-  -- have := lookup_snd_eq_fst_of_mem_support_get_or_else _ _ hx,
-  -- simp [is_cached_of_lookup_eq_some _ this, prod.eq_iff_fst_eq_snd_eq, this]
 end
 
 @[simp_dist_equiv]
